save

red-black-tree.dfy
@@ -6,6 +6,9 @@ datatype Color = Red | Black
 
 datatype RBTree = Empty  | Node (color : Color, value : int, left : RBTree, right : RBTree)
 
+function method elems(t : RBTree) : set<int> {
+	if t == Empty then {} else {t.value} + elems(t.left) + elems(t.right)
+}
 
 class RBTreeRef {
  	ghost var Tree : RBTree
@@ -16,20 +19,88 @@ class RBTreeRef {
 		var parent: RBTreeRef?
 		var color: Color
 		predicate Valid()
-  	reads this, Repr {
-			this in Repr &&
-				Tree.Node? &&
-				Tree.value == value &&
-				Tree.color == color &&
-				(left == null ==> Tree.left.Empty?) &&
-				(right == null ==> Tree.right.Empty?) &&
-				(left != null ==> left in Repr && left.Repr <= Repr && this !in left.Repr &&
-				left.Valid() && left.Tree == Tree.left && left.parent == this) &&
-				(right != null ==> right in Repr && right.Repr <= Repr && this !in right.Repr &&
-				right.Valid() && right.Tree == Tree.right && right.parent == this) &&
-				isWellFormed(Tree)
+  		reads this, Repr {
+				this in Repr &&
+					Tree.Node? &&
+					Tree.value == value &&
+					Tree.color == color &&
+					(left == null ==> Tree.left.Empty?) &&
+					(right == null ==> Tree.right.Empty?) &&
+					(left != null ==> left in Repr && left.Repr <= Repr && this !in left.Repr &&
+					left.Valid() && left.Tree == Tree.left && left.parent == this) &&
+					(right != null ==> right in Repr && right.Repr <= Repr && this !in right.Repr &&
+					right.Valid() && right.Tree == Tree.right && right.parent == this) &&
+					isWellFormed(Tree)
 		}
+
+
+		// termination metric
+		static function ReprN (t : RBTreeRef?) : set<RBTreeRef>
+		reads t {
+			if (t == null) then {} else t.Repr
+		}
+
+		static method Member(t : RBTreeRef?, v : int) returns (r : bool)
+			// requires t != null ==> t.Valid()
+			// decreases ReprN(t)
+		{
+			// if (t == null) {
+			// 	r := false;
+			// }
+
+			// else if (v < t.value) {
+			// 	r := Member(t.left, v);
+			// }
+
+			// else if (v > t.value) {
+			// 	r := Member(t.right, v);
+			// }
+
+			// else {
+			// 	r := true;
+		// }
+		r := true;
+		return true;
+		}
+
+		static method Constant(t :RBTreeRef?) returns (r : bool) {
+			return true;
+		}
+
 }
+
+method Testing()
+{
+	var t0 := Node(Red,10,(Node(Black,9,Empty,Empty)),Empty);
+	assert(!isWellFormed(t0));
+	var t1 := Node(Black,10,(Node(Red,9,Empty,Empty)),Empty);
+	assert(isWellFormed(t1));
+
+	var t2 := new RBTreeRef;
+	t2.Tree := t1;
+	t2.value, t2.color, t2.right, t2.parent := 10, Black, null, null;
+
+	var t3 := new RBTreeRef;
+	t3.Tree := Node(Red,9,Empty,Empty);
+	t3.left := null;
+	t3.right := null;
+	t3.color := Red;
+	t3.parent := t2;
+	t3.value := 9;
+
+	t2.Repr := {t2,t3}	;
+	t3.Repr := {t3};
+	t2.left := t3;
+
+	assert(t2.Valid());
+
+
+	// var r := RBTreeRef.Member(t3, 9);
+	// assert(t2.value == 10);
+
+	var r := RBTreeRef.Constant(null);
+}
+
 
 // predicate isBlack(t : RBTree) {
 // 	!isRed(t)
@@ -49,11 +120,17 @@ predicate isBalanced(t : RBTree) {
 		(countBlack(t.left) == countBlack(t.right) && isBalanced(t.left) && isBalanced(t.right))
 }
 
-predicate isOrdered(t: RBTree) {
+predicate isOrdered(t : RBTree) {
 	if t.Empty? then true else
-		(t.left.Node? ==> t.left.value < t.value && isOrdered(t.left)) &&
-		(t.right.Node? ==> t.value < t.right.value && isOrdered(t.right))
+		(forall i :: i in elems(t.left) ==> i < t.value) &&
+		(forall i :: i in elems(t.right) ==> i > t.value)
 }
+
+// predicate isOrdered(t: RBTree) {
+// 	if t.Empty? then true else
+// 		(t.left.Node? ==> t.left.value < t.value && isOrdered(t.left)) &&
+// 		(t.right.Node? ==> t.value < t.right.value && isOrdered(t.right))
+// }
 
 
 predicate noRedRed(t : RBTree) {
@@ -74,13 +151,6 @@ predicate almostWellFormed(t : RBTree) {
 	isBalanced(t) && isOrdered(t) && noRedRedExceptTop(t)
 }
 
-method Testing()
-{
-	var t0 := Node(Red,10,(Node(Black,9,Empty,Empty)),Empty);
-	assert(!isWellFormed(t0));
-	var t1 := Node(Black,10,(Node(Red,9,Empty,Empty)),Empty);
-	assert(isWellFormed(t1));
-}
 
 
 // method ins(t : RBTree, v: int) returns (r : RBTree)
